src/status.sh
@@ -1,0 +1,3 @@
+#!/bin/bash
+
+egrep -R "admit|Admitted|cheat|give_up|TODO|FIXME" *.v
